\begin{enumerate}[(a)]
    \item Proof as the following:
    \begin{align*}
        \frac{\partial g}{\partial z} &= - \frac{1}{\left(1 + e^{-z}\right)^2 } \cdot \left(e^{-z}\right) \cdot -1 \\
        &= \frac{\left(e^{-z}\right)}{\left(1 + e^{-z}\right)^2} \\
        &= \frac{1}{1+e^{-z}} \cdot \frac{e^{-z}}{1+e^{-z}} \\
        &= g(z)(1-g(z))
    \end{align*}
    \item Proof as follows:
    \begin{align*}
        1 - g(z) &= \frac{e^{-z}}{1+e^{-z}} \\
        &= \frac{1}{e^z + 1} \\
        &= g(-z)
    \end{align*}
\end{enumerate}


